\begin{proof}
  assume $\mathop{d}(x_{n}, z_{n}) \le \epsilon$, and $\mathop{d}(z_{n}, z) \le \alpha_{n}\epsilon$ 

  \[
  \mathop{d}(x_{n+1}, z) \le \mathop{d}(x_{n+1}, z_{n}) + \mathop{d}(z_{n}, z)
  \]

  Notice

  \[
  \mathop{d}(x_{n+1}, z_{n}) = \mathop{d}(f(x_{n}), f(z_{n})) \le \alpha_{n} \mathop{d}(x_{n}, z_{n}) \le \alpha_{n} \epsilon
  \]

  Hence

  \[
  \mathop{d}(x_{n+1}, z) \le 2 \alpha_{n} \epsilon = \beta \epsilon
  \]
\end{proof}

\begin{proof}
  let $x,y \in \mathbb{R}$ than $\mathop{d}(x_{n+1}, y_{n+1}) =
  \mathop{d}(f(x_{n}), f(y_{n})) \le \alpha_{n}\mathop{d}(x_{n}, y_{n})$. With
  induction $\mathop{d}(x_{n}, y_{n}) = \mathop{d}(x_{0}, y_{0})\Pi_{i=0}^{n} \alpha_{i}$

  Hence

  \[
  \lim_{n \rightarrow \infty} \mathop{d}(x_{n}, y_{n}) = \mathop{d}(x_{0}, y_{0})\lim_{n \rightarrow \infty} \Pi_{i=0}^{n} \alpha_{i} = 0
  \]

\end{proof}
